examples/compute/src/bir_computeScript.sml
@@ -1,8 +1,16 @@
 open HolKernel Parse bossLib boolLib
 open bir_basicTheory bir_binexpTheory bir_unaryexpTheory bir_envTheory
+open bir_binpredTheory
 
 
 val _ = new_theory "bir_compute"
+
+Definition bir_compute_ifthenelse_def:
+    bir_compute_ifthenelse b v1 v2 = 
+        if b = SOME birT then v1 
+        else if b = SOME birF then v2
+        else NONE
+End
 
 
 Definition bir_compute_exp_def:
@@ -22,15 +30,15 @@ Definition bir_compute_exp_def:
      bir_compute_binexp et (bir_compute_exp e1 env) (bir_compute_exp e2 env))) /\
 
   (bir_compute_exp (BExp_BinPred pt e1 e2) env = (
-     bir_compute_binpred pt (bir_compute_exp e1 env) (bir_compute_exp e2 env)))
+     bir_compute_binpred pt (bir_compute_exp e1 env) (bir_compute_exp e2 env))) /\
   (**)
   (* (bir_compute (BExp_MemEq e1 e2) env = ( *)
   (*    bir_eval_memeq (bir_compute e1 env) (bir_compute e2 env))) /\ *)
   (**)
   (**)
-  (* (bir_compute (BExp_IfThenElse c et ef) env = *)
-  (*    bir_eval_ifthenelse (bir_compute c env) (bir_compute et env) (bir_compute ef env) *)
-  (* ) /\ *)
+  (bir_compute_exp (BExp_IfThenElse c et ef) env =
+     bir_compute_ifthenelse (bir_compute_exp c env) (bir_compute_exp et env) (bir_compute_exp ef env)
+  )
   (**)
   (* (bir_compute (BExp_Load mem_e a_e en ty) env = *)
   (*    bir_eval_load (bir_compute mem_e env) (bir_compute a_e env) en ty) /\ *)
