examples/compute/src/bir_evalScript.sml
@@ -1,6 +1,6 @@
 open HolKernel Parse bossLib boolLib
 open bir_basicTheory bir_binexpTheory bir_unaryexpTheory bir_envTheory
-open bir_binpred
+open bir_binpredTheory
 
 
 val _ = new_theory "bir_eval"
@@ -34,6 +34,21 @@ Inductive bir_eval_exp:
             (bir_eval_binpred binpred v1 v2 b))
         ==>
         (bir_eval_exp env (BExp_BinPred binpred e1 e2) b))
+
+[~BExp_IfThenElse1:]
+    (!env epred e1 e2 v1 v2.
+        ((bir_eval_exp env epred birT) /\
+            (bir_eval_exp env e1 v1) /\ (bir_eval_exp env e2 v2))
+        ==>
+        (bir_eval_exp env (BExp_IfThenElse epred e1 e2) v1))
+    
+[~BExp_IfThenElse2:]
+    (!env epred e1 e2 v1 v2.
+        ((bir_eval_exp env epred birF) /\
+            (bir_eval_exp env e1 v1) /\ (bir_eval_exp env e2 v2))
+        ==>
+        (bir_eval_exp env (BExp_IfThenElse epred e1 e2) v2))
+
 End
 
 
